\documentclass[UTF8,a4paper,10pt]{article}

\input{preamble.tex}

% \begin{equation*}
%   \begin{aligned}
%   \end{aligned}
% \end{equation*}

% \begin{mybox}{}
% \end{mybox}


% \begin{Problem}[]{}
% \end{Problem}

% \begin{solution}\,
% \end{solution}
  

% \begin{enumerate}[label=(\alph*)]
% \end{enumerate} 

% \setcounter{section}{3} 
% \setcounter{theorem}{3}

% \begin{theorem}\label{thm:3.4}
%   If $E = \bigcup_{k} E_k$ is a countable union of sets, then $|E|_e \leq \sum_{k} |E_k|_e$.
%   \end{theorem}

%  \footcite[][42]{Wheeden_Zygmund_2015}

\begin{document}


% \begin{mybox}{}


% \end{mybox}



% Q1
\section*{Transition Models}

$t_{ij}^{\prime} s$ are assumed to be equally spaced.


Let $H_i=\left\{y_k, k=1, \cdots, j-1\right\}$. 

Consider \[f(y_{ij}\mid H_{ij},\alpha,\beta) = \exp\left\{\frac{y_{ij}-\psi(\theta_{ij})}{\phi}+c(y_{ij},\phi)\right\},\] where \(\psi(\theta_{ij})\) and \(c(y_{ij},\phi)\) are known functions. 

One has 
$$\mu_{ij}^c=E\left[y_{ij} \mid H_{ij}\right]=\psi^{\prime}\left(\theta_{ij}\right)$$ 
and 
$$v_{ij}^c=V\left[y_{ij} \mid H_{ij}\right]=\psi''\left(\theta_{ij}\right) \phi$$ 

with

\[h(\mu_{ij}^c) = x_{ij}^T\beta +\sum_{r=1}^{s}f_r(H_{ij};\alpha)\text{ for suitable functions }f_r(\cdot)'s,\]
and

\[v_{ij}^c = v(\mu_{ij}^c)\phi.\]


\begin{Problem}[]{Fitting transition models: (A markov model of order $q$ )}


By
\[L_i(y_{i1},\cdots,y_{im_i}) = f(y_{i1},\cdots,y_{iq})\prod_{j=q+1}^{m_i}f(y_{ij}\mid y_{i\, j-1},\cdots,y_{i \, j-q}), i = 1,\cdots,n,\]

one can get the likelihood function 

\[L(\alpha,\beta) = \prod_{i=1}^{n}f(y_{i1},\cdots,y_{iq})\prod_{j=q+1}^{m_i}f(y_{ij}\mid H_{ij},\alpha,\beta),\]
where 

\[H_{ij} = \{y_{i \, j-1},\cdots,y_{i \, j-q}\}.\]

Since the term $f\left(y_{i1}, \cdots, y_{iq}\right)$ is always unavailable, the estimators of $(\alpha, \beta)$ are obtained via maximizing the conditional likelihood 

$$\prod_{i=1}^{n} \prod_{j=q+1}^{m_i} f\left(y_{ij}\mid H_{ij}, \alpha, \beta\right).$$

Let $\theta=(\alpha, \beta)$.

Show that the log-conditional likelihood or conditional score function has the form

\[S^c(\theta) = \sum_{i=1}^{n}\sum_{j = (q+1)}^{m_i}\frac{\partial \mu_{ij}^c}{\partial \theta}{v_{ij}^c}^{-1}(y_{ij}-\mu_{ij}^c).\]

\end{Problem}


\[L^c(\theta) =  \prod_{i=1}^{n} \prod_{j=q+1}^{m_i} f\left(y_{ij}\mid H_{ij}, \alpha, \beta\right).\]

\[l^c(\theta) = \ln L^c(\theta) = \dfrac{\sum_{i=1}^{n}\sum_{j = (q+1)}^{m_i}(y_{ij}\theta_{ij}-\psi(\theta_{ij}))}{\phi}+\sum_{i=1}^{n}\sum_{j = (q+1)}^{m_i}c(y_{ij},\phi).\]


We have
\begin{align*}
  S^c(\theta) = \frac{\partial l^c(\theta)}{\partial \theta} &= \frac{\sum_{i=1}^{n}\sum_{j = (q+1)}^{m_i}(y_{ij}-\psi'(\theta_{ij}))}{\phi}\\
  & = \sum_{i=1}^{n}\sum_{j = (q+1)}^{m_i} \frac{1}{\phi} (y_{ij}-\mu_{ij}^c)\\
  & = \sum_{i=1}^{n}\sum_{j = (q+1)}^{m_i}\frac{\partial \mu_{ij}^c}{\partial \theta}{v_{ij}^c}^{-1}(y_{ij}-\mu_{ij}^c),
\end{align*}


where
\begin{align*}
\E[y_{ij}\mid H_{ij}] = \psi'(\theta_{ij}) &\triangleq \mu_{ij}^c,\\
\V[y_{ij}\mid H_{ij}] = \psi''(\theta_{ij}) \phi
 = \frac{\partial \mu_{ij}^c}{\partial\theta}\phi &\triangleq v_{ij}^c \implies \frac{1}{\phi} = \frac{\partial \mu_{ij}^c}{\partial\theta} {v_{ij}^c}^{-1}.
\end{align*}




\pagebreak

\begin{Problem}[]{
Ordered Categorical data}


$Y$: ordinal response with categories labeled $1,2, \cdots, k$.


Let $$F(a \mid x)=P(Y \leq a \mid x),$$ where $a=1, \cdots,(k-1), x=\left(x_1, \cdots, x_p\right)^T$.

Proportional odds model: $$\logit F(a \mid x)=\theta_a+x^T \beta,\quad a=1, \cdots,(k-1).$$

Define $Y^*=\left(Y_1^*, \cdots, Y_{k-1}^*\right)$ with $Y_a^*=1_{(Y\leq a)}$. 

Then, $$\logit F(a \mid x)=\logit P\left(Y_a^*=1 \mid x\right).$$



\begin{center}
\begin{tabular}{c|cccccc}
    
    $Y$ & 1 & 2 & 3 & $\cdots$ & $k-1$ & $k$ \\
    \hline$Y_1^*$ & 1 & 0 & 0 & $\cdots$ & 0 & 0 \\
    $Y_2^*$ & 1 & 1 & 0 & $\cdots$ & 0 & 0 \\
    $\vdots$ & $\vdots$ & $\vdots$ & & & & $\vdots$ \\
    $Y_{k-1}^*$ & 1 & 1 & 1 & $\cdots$ & 1 & 0
  \end{tabular}
\end{center}


\dotfill


Example:


Assume that $$\logit P\left(Y_j \leq b \mid Y_{i \, j-1}=a\right)=\theta_{ab}+x_i{ }^T \beta_{a}, \quad a, b=1, \cdots,(k-1).$$ 

It can be derived that

\[\logit P(Y_{ij}\leq b\mid Y_{i\,j-1}^* = y_{i\,j-1}^*) = \theta_b +\sum_{l=1 }^{k-1}\alpha_{lb}y_{i(j-1)l}^*+x_{ij}^T(\beta +\sum_{l=1}^{k-1}r_{l}y_{i(j-1)l}^*),\]

where
$\left\{\begin{array}{l}
\theta_{kb} = \theta_b,\\
\alpha_{lb} = \theta_{lb}-\theta_{l+1\,b},\\
\beta_k = \beta,\\
r_{l} = \beta_{l}-\beta_{l+1}
\end{array}\right..$


\end{Problem}

\pagebreak

\begin{align*}
  Y_{ij} &= a\\
   \Rightarrow  Y_{ij}^* &= (\underset{a-1}{\underbrace{0\,\cdots\,0}} \,\, \underset{k-a}{\underbrace{1\,\cdots\,1}}).
\end{align*}

\begin{align*}
  % &\,
  \logit P(Y_{ij}\leq b\mid Y_{i\,j-1}^* = y_{i\,j-1}^*) 
  = \theta_b + & (\theta_{1b}-\theta_{2\,b})y_{i(j-1)1}^*  &+ x_{ij}^T\{    \beta&+(\beta_{1}-\beta_{2})y_{i(j-1)1}^*\\
  +&(\theta_{2b}-\theta_{3\,b})y_{i(j-1)2}^* &&+ (\beta_{2}-\beta_{3})y_{i(j-1)2}^*\\
  +&\cdots  &&+\cdots\\
  +&(\theta_{a-1\,b}-\theta_{ab})y_{i(j-1)(a-1)}^* &&+(\beta_{a-1}-\beta_{a})y_{i(j-1)(a-1)}^*\\
  +&(\theta_{ab}-\theta_{a+1\,b})y_{i(j-1)a}^* && +(\beta_{a}-\beta_{a+1})y_{i(j-1)a}^*\\
  +&(\theta_{a+1\,b}-\theta_{a+2\,b})y_{i(j-1)(a+1)}^* && +(\beta_{a+1}-\beta_{a+2})y_{i(j-1)(a+1)}^*\\
  +&\cdots &&+\cdots\\
  +&(\theta_{(k-1)b}-\theta_{k\,b})y_{i(j-1)(k-1)}^* && +(\beta_{k-1}-\beta_{k})y_{i(j-1)(k-1)}^*\}.
\end{align*}

\begin{align*}
  % &\,
  \logit P(Y_{ij}\leq b\mid Y_{i \, j-1} = a)  
  =\theta_b +&(\theta_{ab}-\theta_{a+1\,b}) & + x_{ij}^T\{    \beta& +(\beta_{a}-\beta_{a+1})\\
  +&(\theta_{a+1\,b}-\theta_{a+2\,b}) && +(\beta_{a+1}-\beta_{a+2})\\
  +&\cdots &&+\cdots\\
  +&(\theta_{(k-1)b}-\theta_{k\,b}) && +(\beta_{k-1}-\beta_{k})\}.
\end{align*}

\begin{align*}
  % &\,
  \logit P(Y_{ij}\leq b\mid Y_{i \, j-1} = a)  
  &=\theta_b +\theta_{ab}-\theta_{kb} + x_{ij}^T\{\beta +\beta_{a}-\beta_{k}\}\\
  &=\theta_{ab}+x_{ij}^T\beta_{a}.
\end{align*}


\pagebreak

\begin{Problem}[]{Log-linear transition models for count data}


 
$Y_{ij} \mid\left(H_{ij}, x_{ij}\right) \sim$ Poissom $\left(\mu^c_{ij}\right)$.

\dotfill

Model 1. Wong (1986) proposed that $$\mu_{ij}^c=\exp \left(x_{ij}^T\beta\right) \{1+\exp \left(-\alpha_0-\alpha_1 y_{i\,j-1}\right)\},$$ 

$\alpha_0, \alpha_1>0$, where $\beta$ is the influence of $x_{ij}$ as $y_{i\,j-1}=0$.

---

Remark. When $y_{i\,j-1}>0, \mu_{ij}^c$ decreases as $y_{i\,j-1}$ increases. A negative association is implied between the prior and current responses.

\dotfill

Model 2. $\mu_{ij}^c=\exp \left(x_{ij}^T\beta+\alpha y_{i\,j-1}\right)$.

---

Properties: 
\begin{enumerate}
  \item $\mu_{ij}^c$ increases as an exponential function of time as $\alpha>0$.
  \item When $\exp \left(x_{ij}^T \beta\right)=\mu$ and $\alpha<0$, it leads to a stationary process.
\end{enumerate}

\end{Problem}

\begin{align*}
  \E[Y_{ij} \mid\left(H_{ij}, x_{ij}\right)] = 、Var[Y_{ij} \mid\left(H_{ij}, x_{ij}\right)] = \mu_{ij}^c.
\end{align*}
We can obtain
\begin{align*}
  \E[Y_{ij}] = \E[\mu_{ij}^c] &= \E[\exp\left(x_{ij}^T\beta+\alpha y_{i\,j-1}\right)]\\
  &=\exp\left(x_{ij}^T\beta\right)\E[\exp\left(\alpha y_{i\,j-1}\right)]\\
  &=\mu\E[\exp\left(\alpha y_{i\,j-1}\right)]
\end{align*}
If stationary, 
\begin{align*}
  \mu = \mu  \exp\left(\alpha \mu\right)\\
\end{align*}

\pagebreak

\begin{Problem}[]{   }


   Moded 3. $$\mu_{ij}=\exp \left(x_{ij}{ }^T \beta+\alpha\left\{\ln \left(y_{i\,j-1}^*\right)-x_{i\,j-1}^T \beta\right\}\right),$$ 

where $y_{i\,j-1}^*=\max \left\{y_{i\,j-1}, d\right\}, 0<d<1$.

---

Property: $\left\{\begin{array}{l}\alpha=0 \text { : it reduces to an oedinary log-tinear model. } \\ \alpha<0 \text { : negative correlation between } y_{i\,j-1} \text { and } y_{ij} \\ 
  \alpha>0 \text { : positive correlation between } y_{i\,j-1} \text { and } y_{ij}\end{array}\right.$

  ---

  Application to a size-independent branching process:

   \(\exp(x_{ij}^T\beta) = \mu\)

   \begin{conditions}
    y_{ij}     & :      &  the number of individuals in the \(i\)-th population at generation \(j\) \\
    Z_{k}(y_{i\,j-1})     & :      &  the number of offspring for person \(k\) in generation \((j-1)\)
   \end{conditions}

   For \(y_{i\,j-1}>0,\)
   \[y_{ij} =\sum_{k=1}^{y_{i(j-1)}}Z_k(y_{i(j-1)}),\]
where 
\[Z_{k}\overset{iid}{\sim}Poisson\left(\left(\frac{\mu}{y_{i{j-1}}^*}\right)^{1-\alpha}\right).\]

One can get 


\[\mu_{ij}^c = \mu\cdot\left(\frac{y_{i(j-1)}}{\mu}\right)^\alpha.\]

Property:

\begin{itemize}
  \item \(\alpha<0\): the sample paths oscillate back and forth about their long-term average level.
  \item \(\alpha>0\): the sample paths have sharper peaks and broader valleys.
\end{itemize}

  \end{Problem}

\includepdf[pages=-]{R10A21126_HW05_Q4.pdf}



\end{document}

